Plfl/DeBruijn.lean
@@ -10,7 +10,7 @@ inductive Context : Type
   | cons : Context → Ty → Context
 
 notation "∅" => Context.empty
-notation:50 Γ ";" τ => Context.cons Γ τ
+notation:40 Γ ";" τ:50 => Context.cons Γ τ
 
 inductive Lookup : Context → Ty → Prop
   | here {Γ τ} : Lookup (Γ ; τ) τ
@@ -18,39 +18,59 @@ inductive Lookup : Context → Ty → Prop
 
 notation:40 Γ "∋" τ:40 => Lookup Γ τ
 
-inductive Judgement : Context → Ty → Type
-  | var {Γ τ} : Γ ∋ τ → Judgement Γ τ
-  | app {Γ τ τ'} : Judgement Γ (τ ⇒ τ') → Judgement Γ τ → Judgement Γ τ'
-  | lam {Γ τ τ'} : Judgement (Γ ; τ) τ' → Judgement Γ (τ ⇒ τ')
-  | tru {Γ} : Judgement Γ bool
-  | fls {Γ} : Judgement Γ bool
-  | ite {Γ τ} : Judgement Γ bool → Judgement Γ τ → Judgement Γ τ → Judgement Γ τ
+inductive Typing : Context → Ty → Type
+  | var {Γ τ} : Γ ∋ τ → Typing Γ τ
+  | app {Γ τ τ'} : Typing Γ (τ ⇒ τ') → Typing Γ τ → Typing Γ τ'
+  | lam {Γ τ τ'} : Typing (Γ ; τ) τ' → Typing Γ (τ ⇒ τ')
+  | tru {Γ} : Typing Γ bool
+  | fls {Γ} : Typing Γ bool
+  | ite {Γ τ} : Typing Γ bool → Typing Γ τ → Typing Γ τ → Typing Γ τ
 
-notation:40 Γ "⊢" τ:40 => Judgement Γ τ
-notation "true"  => Judgement.tru
-notation "false" => Judgement.fls
-prefix:90 "$ "   => Judgement.var
-notation:50 "λ" t:50 => Judgement.lam t
-infix:70 " ⬝ "   => Judgement.app
-notation "if" c "then" t₁ "else" t₂ => Judgement.ite c t₁ t₂
+notation:40 Γ "⊢" τ:50 => Typing Γ τ
+notation "true"  => Typing.tru
+notation "false" => Typing.fls
+prefix:90 "` "   => Typing.var
+notation:60 "λ" t:60 => Typing.lam t
+infixl:70 " ⬝ "   => Typing.app
+notation:60 "if" c "then" t₁ "else" t₂ => Typing.ite c t₁ t₂
 
-def length : Context → Nat
+def Context.length : Context → Nat
   | Context.empty => 0
   | Context.cons Γ _ => length Γ + 1
 
-def lookup : ∀ {Γ : Context} {n : Nat}, (h : n < length Γ) → Ty
+def lookup : ∀ {Γ : Context} {n : Nat}, (h : n < Γ.length) → Ty
   | Context.cons _ τ,     0, _ => τ
-  | Context.cons _ _, _ + 1, h => lookup (Nat.lt_of_succ_lt h)
+  | Context.cons _ _, _ + 1, h => lookup (Nat.lt_of_succ_lt_succ h)
 
-def count : ∀ {Γ : Context} {n : Nat}, (h : n < length Γ) → Γ ∋ lookup h
-  | Context.cons _ τ,     0, _ => Lookup.here
-  | Context.cons _ _, _ + 1, h => Lookup.there (count (Nat.lt_of_succ_lt h))
+def count : ∀ {Γ : Context} {n : Nat}, (h : n < Γ.length) → Γ ∋ lookup h
+  | Context.cons _ _,     0, _ => Lookup.here
+  | Context.cons _ _, _ + 1, h => Lookup.there (count (Nat.lt_of_succ_lt_succ h))
+
 /-
 def ex : ∅ ⊢ (bool ⇒ bool) ⇒ bool ⇒ bool
   := λ λ (ref 1 · (ref 1 · ref 0))
 -/
 
-def ref {Γ : Context} : (n : Nat) → (h : n + 1 < length Γ) → Γ ∋ lookup h
-  | _ , h => count h
+def lookup_at {Γ : Context} : (n : Nat) → {h : n < Γ.length} → Γ ⊢ lookup h
+  | _ , h => ` count h
 
-def ex : ∅ ⊢ (bool ⇒ bool) ⇒ bool ⇒ bool := by sorry
+prefix:90 "# " => lookup_at
+
+/- def ex : ∅ ⊢ (bool ⇒ bool) ⇒ bool ⇒ bool :=
+  λ λ (# 1 ⬝ (# 1 ⬝ # 0)) -/
+
+theorem extend {Γ Δ} : (∀ {τ}, Γ ∋ τ → Δ ∋ τ)
+  → ∀ {τ τ'}, Γ; τ' ∋ τ → Δ; τ' ∋ τ := by
+    intros ρ τ τ' h
+    cases h with
+    | here => apply Lookup.here
+    | there h => apply Lookup.there (ρ h)
+
+theorem rename {Γ Δ} : (∀ {τ}, Γ ∋ τ → Δ ∋ τ) → (∀ {τ}, Γ ⊢ τ → Δ ⊢ τ)
+  | ρ, _, Typing.var h => Typing.var (ρ h)
+  | ρ, _, Typing.app t₁ t₂ => Typing.app (rename ρ t₁) (rename ρ t₂)
+  | ρ, _, Typing.lam t => Typing.lam (rename (extend ρ) t)
+  | _, _, Typing.tru => Typing.tru
+  | _, _, Typing.fls => Typing.fls
+  | ρ, _, Typing.ite c t₁ t₂ => Typing.ite (rename ρ c) (rename ρ t₁) (rename ρ t₂)
+
